Fix ml_optimise for fun big step
This optimisation doesn't work with the current setup because it
decreases the clock ticks.

(fn x => exp) y --> let x = y in exp

and the simple theorem about the bottom-up optimiser requires the clock
ticks to be the same.

translator/ml_optimiseScript.sml
@@ -1,11 +1,11 @@
-open HolKernel Parse boolLib bossLib;
-val _ = new_theory "ml_optimise";
+open preamble;
 local open intLib in end;
-open astTheory libTheory semanticPrimitivesTheory bigStepTheory;
+open astTheory libTheory semanticPrimitivesTheory;
 open terminationTheory;
-open evalPropsTheory bigClockTheory determTheory;
 open arithmeticTheory listTheory combinTheory pairTheory;
 open integerTheory ml_translatorTheory lcsymtacs;
+
+val _ = new_theory "ml_optimise";
 
 infix \\ val op \\ = op THEN;
 
@@ -53,7 +53,8 @@ val BOTTOM_UP_OPT_def = tDefine "BOTTOM_UP_OPT" `
   (* TODO: Handle wasn't optimised before full-blown exceptions were in the
            language, but perhaps it should be now? *)
   (BOTTOM_UP_OPT f (Handle x ys) = Handle x ys) /\
-  (BOTTOM_UP_OPT f (Letrec z1 z2) = f (Letrec z1 z2))`
+  (BOTTOM_UP_OPT f (Letrec z1 z2) = f (Letrec z1 z2)) ∧
+  (BOTTOM_UP_OPT f (Tannot x t) = Tannot (BOTTOM_UP_OPT f x) t)`
  (WF_REL_TAC `measure (exp_size o SND)` THEN REPEAT STRIP_TAC
   THEN IMP_RES_TAC MEM_exp_size1 THEN IMP_RES_TAC MEM_exp_size2 THEN DECIDE_TAC)
 
@@ -77,89 +78,99 @@ val do_log_IMP_3 = prove(
 
 val s = ``s:'ffi state``
 
+val map_sing_lemma = Q.prove (
+`[f x] = MAP f [x]`,
+rw []);
+
+val lemma2 = Q.prove(
+`(\a. f x a) = f x`,
+ rw [FUN_EQ_THM]);
+
 val BOTTOM_UP_OPT_LEMMA = prove(
-  ``(!ck env ^s exp res. evaluate F env s exp res ==> isRval (SND res) ==> evaluate F env s (f exp) res) ==>
-    (!ck x1 ^s x2 x3. evaluate ck x1 s x2 x3 ==> isRval (SND x3) ∧ (ck = F) ==> evaluate ck x1 s (BOTTOM_UP_OPT f x2) x3) /\
-    (!ck x1 ^s x2 x3. evaluate_list ck x1 s x2 x3 ==> isRval (SND x3) ∧ (ck = F) ==> evaluate_list ck x1 s (MAP (BOTTOM_UP_OPT f) x2) x3) /\
-    (!ck x1 ^s x2 x3 x4 x5. evaluate_match ck x1 s x2 x3 x4 x5 ==> isRval (SND x5) ∧ (ck = F) ==> evaluate_match ck x1 s x2 (MAP (\(p,x). (p,BOTTOM_UP_OPT f x)) x3) x4 x5)``,
+  ``(!^s env exp res. evaluate s env exp = res ==> isRval (SND res) ==> evaluate s env (MAP f exp) = res) ==>
+    (!^s x1 x2 x3. evaluate s x1 x2 = x3 ==> isRval (SND x3) ==> evaluate s x1 (MAP (BOTTOM_UP_OPT f) x2) = x3) /\
+    (!^s x1 x2 x3 x4 x5. evaluate_match s x1 x2 x3 x4 = x5 ==> isRval (SND x5) ==> evaluate_match s x1 x2 (MAP (\(p,x). (p,BOTTOM_UP_OPT f x)) x3) x4 = x5)``,
   STRIP_TAC \\ ONCE_REWRITE_TAC [two_assums]
-  \\ HO_MATCH_MP_TAC bigStepTheory.evaluate_ind \\ REPEAT STRIP_TAC
-  \\ FULL_SIMP_TAC std_ss [BOTTOM_UP_OPT_def,isRval_def,AND_IMP_INTRO, rich_listTheory.MAP_REVERSE]
-  \\ CONV_TAC (DEPTH_CONV ETA_CONV) \\ ASM_SIMP_TAC std_ss []
-  \\ TRY (ASM_SIMP_TAC (srw_ss()) [Once evaluate_cases] THEN NO_TAC)
-  \\ TRY (Q.PAT_ASSUM `!x.bbb` (fn th => MATCH_MP_TAC th THEN ASSUME_TAC th)
-          THEN ASM_SIMP_TAC (srw_ss()) [Once evaluate_cases,isRval_def] THEN NO_TAC)
-  THEN1 (ASM_SIMP_TAC (srw_ss()) [Once evaluate_cases,isRval_def] \\ METIS_TAC [])
-  THEN1 (ASM_SIMP_TAC (srw_ss()) [Once evaluate_cases,isRval_def] \\ METIS_TAC [])
-  THEN1 (Q.PAT_ASSUM `!x.bbb` (fn th => MATCH_MP_TAC th \\ ASSUME_TAC th)
-    \\ ASM_SIMP_TAC (srw_ss()) [Once evaluate_cases,isRval_def]
-    \\ METIS_TAC [])
-  THEN1 (ASM_SIMP_TAC (srw_ss()) [Once evaluate_cases,isRval_def] \\ METIS_TAC [])
-  THEN1 (Q.PAT_ASSUM `!x.bbb` (fn th => MATCH_MP_TAC th \\ ASSUME_TAC th)
-    \\ ASM_SIMP_TAC (srw_ss()) [Once evaluate_cases,isRval_def]
-    \\ REPEAT DISJ1_TAC \\ METIS_TAC [])
-  THEN1
-   (ASM_SIMP_TAC (srw_ss()) [Once evaluate_cases,isRval_def]
-    \\ REPEAT DISJ1_TAC
-    \\ METIS_TAC [])
-  THEN1
-   (ASM_SIMP_TAC (srw_ss()) [Once evaluate_cases,isRval_def]
-    \\ DISJ2_TAC \\ DISJ1_TAC
-    \\ METIS_TAC [])
-  THEN1
-   (ASM_SIMP_TAC (srw_ss()) [Once evaluate_cases,isRval_def]
-    \\ DISJ2_TAC \\ DISJ1_TAC
-    \\ METIS_TAC [])
-  THEN1 (Q.PAT_ASSUM `!x.bbb` (fn th => MATCH_MP_TAC th \\ ASSUME_TAC th)
-    \\ ASM_SIMP_TAC (srw_ss()) [Once evaluate_cases,isRval_def]
-    \\ REPEAT DISJ1_TAC \\ METIS_TAC [])
-  THEN1
-   (ASM_SIMP_TAC (srw_ss()) [Once evaluate_cases,isRval_def]
-    \\ REPEAT DISJ1_TAC
-    \\ METIS_TAC [])
-  THEN1
-   (ASM_SIMP_TAC (srw_ss()) [Once evaluate_cases,isRval_def]
-    \\ DISJ2_TAC \\ DISJ1_TAC
-    \\ METIS_TAC [])
-  THEN1
-   (Q.PAT_ASSUM `!x.bbb` (fn th => MATCH_MP_TAC th \\ ASSUME_TAC th) \\ fs []
-    \\ ASM_SIMP_TAC (srw_ss()) [Once evaluate_cases,isRval_def]
-    \\ Cases_on `x3` \\ fs [] \\ IMP_RES_TAC do_log_IMP \\ SRW_TAC [] []
-    \\ Cases_on `r` \\ fs [isRval_def] \\ METIS_TAC [do_log_IMP_2])
-  THEN1 (ASM_SIMP_TAC (srw_ss()) [Once evaluate_cases,isRval_def] \\ METIS_TAC [])
-  THEN1
-   (Q.PAT_ASSUM `!x.bbb` (fn th => MATCH_MP_TAC th \\ ASSUME_TAC th) \\ fs []
-    \\ ASM_SIMP_TAC (srw_ss()) [Once evaluate_cases,isRval_def]
-    \\ METIS_TAC [do_log_IMP_3])
-  THEN1 (ASM_SIMP_TAC (srw_ss()) [Once evaluate_cases,isRval_def] \\ METIS_TAC [])
-  THEN1 (ASM_SIMP_TAC (srw_ss()) [Once evaluate_cases,isRval_def] \\ METIS_TAC [])
-  \\ TRY (Q.PAT_ASSUM `!x.bbb` (fn th => MATCH_MP_TAC th \\ ASSUME_TAC th))
-  THEN1
-   (ASM_SIMP_TAC (srw_ss()) [Once evaluate_cases,isRval_def] \\ fs [do_if_def]
-    \\ Cases_on `v = Boolv T` \\ Cases_on `v = Boolv F` \\ fs [Boolv_11]
-    THEN1 METIS_TAC []
-    \\ SRW_TAC [] [] \\ Cases_on `x3` \\ fs [] \\ Cases_on `r` \\ fs [isRval_def]
-    \\ METIS_TAC [Boolv_11])
-  \\ ASM_SIMP_TAC (srw_ss()) [Once evaluate_cases,isRval_def] \\ METIS_TAC []);
+  \\ HO_MATCH_MP_TAC evaluate_ind
+  >> rw [evaluate_def, BOTTOM_UP_OPT_def]
+  >> simp_tac std_ss [Once map_sing_lemma]
+  >> TRY (first_assum irule)
+  >> simp [evaluate_def]
+  >- (
+    every_case_tac
+    >> fs [isRval_def]
+    >> rw [])
+  >- (
+    every_case_tac
+    >> fs [isRval_def]
+    >> rw []
+    >> fs [rich_listTheory.MAP_REVERSE, lemma2]
+    >> rw []
+    >> fs [])
+  >- (
+    every_case_tac
+    >> fs [isRval_def]
+    >> rw []
+    >> fs [rich_listTheory.MAP_REVERSE, lemma2]
+    >> rw []
+    >> fs [])
+  >- (
+    Cases_on `evaluate s x1 [e1]`
+    >> Cases_on `r`
+    >> fs []
+    >> Cases_on `do_log lop (HD a) e2`
+    >> fs [isRval_def]
+    >> Cases_on `x`
+    >> fs []
+    >> TRY (drule do_log_IMP)
+    >> TRY (drule do_log_IMP_3)
+    >> rw []
+    >> drule do_log_IMP_2
+    >> rw [])
+  >- (
+    every_case_tac
+    >> fs [isRval_def]
+    >> rw []
+    >> fs [do_if_def]
+    >> Cases_on `HD a = Boolv T`
+    >> Cases_on `HD a = Boolv F`
+    >> fs [Boolv_11]
+    >> rw [])
+  >- (
+    every_case_tac
+    >> fs [isRval_def]
+    >> rw [])
+  >- (
+    every_case_tac
+    >> fs [isRval_def]
+    >> rw [])
+  >- (
+    every_case_tac
+    >> fs [isRval_def]
+    >> rw []));
 
 val BOTTOM_UP_OPT_THM = prove(
   ``!f.
-      (!env ^s exp t res.
-         evaluate F env s exp (t,Rval res) ==>
-         evaluate F env s (f exp) (t,Rval res)) ==>
-      (!env ^s exp t res.
-         evaluate F env s exp (t,Rval res) ==>
-         evaluate F env s (BOTTOM_UP_OPT f exp) (t,Rval res))``,
+      (!^s env exp t res.
+         evaluate s env exp = (t,Rval res) ==>
+         evaluate s env (MAP f exp) = (t,Rval res)) ==>
+      (!^s env exp t res.
+         evaluate s env exp = (t,Rval res) ==>
+         evaluate s env (MAP (BOTTOM_UP_OPT f) exp) = (t,Rval res))``,
   STRIP_TAC \\ STRIP_TAC \\ (BOTTOM_UP_OPT_LEMMA
     |> UNDISCH |> CONJUNCT1
-    |> Q.SPECL [`F`, `env`,`s`,`exp`,`(t,Rval res)`] |> GEN_ALL
+    |> Q.SPECL [`s`, `env`,`exp`,`(t,Rval res)`] |> GEN_ALL
     |> DISCH_ALL |> GEN_ALL |> SIMP_RULE std_ss [isRval_def] |> MATCH_MP_TAC)
-  \\ REPEAT STRIP_TAC \\ Cases_on `res` \\ FULL_SIMP_TAC std_ss [isRval_def]
+  \\ REPEAT STRIP_TAC \\ Cases_on `evaluate s env exp` \\ FULL_SIMP_TAC std_ss [isRval_def]
   \\ Cases_on `r` \\ FULL_SIMP_TAC std_ss [isRval_def])
   |> SIMP_RULE std_ss [PULL_FORALL,AND_IMP_INTRO];
 
 
 (* rewrite optimisation: (fn x => exp) y --> let x = y in exp *)
+
+(*
+ * TODO: This optimisation changes the clock ticks, and so needs a more complicated
+ * setup
 
 val abs2let_def = Define `
   abs2let x =
@@ -167,23 +178,20 @@ val abs2let_def = Define `
              | rest => rest`;
 
 val abs2let_thm = prove(
-  ``!env s exp t res. evaluate F env s exp (t,Rval res) ==>
-                      evaluate F env s (abs2let exp) (t,Rval res)``,
+  ``!s env exp t res. evaluate s env [exp] = (t,Rval res) ==>
+                      evaluate s env [abs2let exp] = (t,Rval res)``,
+
   SIMP_TAC std_ss [abs2let_def] \\ REPEAT STRIP_TAC
   \\ BasicProvers.EVERY_CASE_TAC
   \\ ASM_SIMP_TAC std_ss [] \\ POP_ASSUM MP_TAC
-  \\ SIMP_TAC (srw_ss()) [Once evaluate_cases,do_opapp_def]
-  \\ REPEAT STRIP_TAC \\ SIMP_TAC (srw_ss()) [Once evaluate_cases]
+  \\ SIMP_TAC (srw_ss()) [evaluate_def,do_opapp_def]
+  \\ REPEAT STRIP_TAC \\ SIMP_TAC (srw_ss()) [evaluate_def]
   \\ BasicProvers.EVERY_CASE_TAC
   \\ SRW_TAC [] []
-  \\ NTAC 3 (FULL_SIMP_TAC (srw_ss()) [Once (hd (tl (CONJUNCTS evaluate_cases)))])
-  \\ first_assum(preamble.match_exists_tac o concl)
-  \\ FULL_SIMP_TAC std_ss []
-  \\ Q.PAT_ASSUM `evaluate F env s (Fun s' e) ((s2',Rval v1))` MP_TAC
-  \\ SIMP_TAC (srw_ss()) [Once evaluate_cases]
-  \\ REPEAT STRIP_TAC
-  \\ FULL_SIMP_TAC (srw_ss()) [opt_bind_def, SWAP_REVERSE_SYM]
-  \\ METIS_TAC []);
+  >> fs []
+  >> rw [opt_bind_def]
+  >> fs [evaluateTheory.dec_clock_def]);
+  *)
 
 (* rewrite optimisation: let x = y in x --> y *)
 
@@ -193,16 +201,16 @@ val let_id_def = Define `
   (let_id rest = rest)`;
 
 val let_id_thm = prove(
-  ``!env s exp t res. evaluate F env s exp (t,Rval res) ==>
-                      evaluate F env s (let_id exp) (t,Rval res)``,
+  ``!s env exp t res. evaluate s env [exp] = (t,Rval res) ==>
+                      evaluate s env [let_id exp] = (t,Rval res)``,
   STRIP_TAC \\ STRIP_TAC \\ HO_MATCH_MP_TAC (fetch "-" "let_id_ind")
   \\ FULL_SIMP_TAC std_ss [let_id_def] \\ SRW_TAC [] [] \\ POP_ASSUM MP_TAC
-  \\ SIMP_TAC (srw_ss()) [Once evaluate_cases]
-  \\ REPEAT STRIP_TAC \\ POP_ASSUM MP_TAC
-  \\ SIMP_TAC (srw_ss()) [Once evaluate_cases]
-  \\ REPEAT STRIP_TAC
-  \\ FULL_SIMP_TAC (srw_ss()) [lookup_var_id_def,opt_bind_def]);
-
+  \\ SIMP_TAC (srw_ss()) [evaluate_def]
+  \\ FULL_SIMP_TAC (srw_ss()) [lookup_var_id_def,opt_bind_def]
+  >> every_case_tac
+  >> rw []
+  >> imp_res_tac evaluatePropsTheory.evaluate_sing
+  >> fs []);
 
 (* rewrite optimisations: x - n + n --> x and x + n - n --> x *)
 
@@ -231,26 +239,25 @@ val dest_binop_thm = prove(
 val do_app_IMP = prove(
   ``(do_app s (Opn opn) [v1; v2] = SOME (s1,e3)) ==>
     ?i1 i2. (v1 = Litv (IntLit i1)) /\ (v2 = Litv (IntLit i2))``,
-  Cases_on`s` >> FULL_SIMP_TAC (srw_ss()) [do_app_cases]
+  Cases_on`s` >> FULL_SIMP_TAC (srw_ss()) [semanticPrimitivesPropsTheory.do_app_cases]
   \\ SRW_TAC [] []);
 
 val evaluate_11_Rval = prove(
-  ``evaluate ck env s exp (t,Rval res1) ==>
-    evaluate ck env s exp (t,Rval res2) ==> (res1 = res2)``,
-  REPEAT STRIP_TAC \\ IMP_RES_TAC big_exp_determ
-  \\ FULL_SIMP_TAC (srw_ss()) []);
+  ``evaluate s env exp = (t,Rval res1) ==>
+    evaluate s env exp = (t,Rval res2) ==> (res1 = res2)``,
+  rw []);
 
 val evaluate_Lit = prove(
-  ``evaluate ck env s (Lit l) (s1,Rval (res)) <=> (res = Litv l) /\ (s = s1)``,
-  FULL_SIMP_TAC (srw_ss()) [Once evaluate_cases] \\ METIS_TAC []);
+  ``evaluate s env [Lit l] = (s1,Rval (res)) <=> (res = [Litv l]) /\ (s = s1)``,
+  FULL_SIMP_TAC (srw_ss()) [evaluate_def] \\ METIS_TAC []);
 
 val with_same_refs_io = Q.prove(
   `x with <| refs := x.refs; ffi := x.ffi |> = x`,
   rw[state_component_equality])
 
 val opt_sub_add_thm = prove(
-  ``!env s exp t res. evaluate F env s exp (t,Rval res) ==>
-                      evaluate F env s (opt_sub_add exp) (t,Rval res)``,
+  ``!s env exp t res. evaluate s env [exp] = (t,Rval res) ==>
+                      evaluate s env [opt_sub_add exp] = (t,Rval res)``,
   STRIP_TAC \\ STRIP_TAC \\ STRIP_TAC \\ SIMP_TAC std_ss [opt_sub_add_def]
   \\ Cases_on `dest_binop exp` \\ FULL_SIMP_TAC std_ss []
   \\ `?x1 x2 x3. x = (x1,x2,x3)` by METIS_TAC [PAIR] \\ fs []
@@ -261,42 +268,58 @@ val opt_sub_add_thm = prove(
   \\ Cases_on `x3 = Lit l` \\ FULL_SIMP_TAC std_ss []
   \\ IMP_RES_TAC dest_binop_thm \\ FULL_SIMP_TAC std_ss []
   \\ SRW_TAC [] [] \\ POP_ASSUM MP_TAC
-  \\ SIMP_TAC (srw_ss()) [Once evaluate_cases]
-  \\ NTAC 3 (FULL_SIMP_TAC (srw_ss()) [Once (hd (tl (CONJUNCTS evaluate_cases)))])
-  \\ fs [PULL_EXISTS]
-  \\ SIMP_TAC (srw_ss()) [Once evaluate_cases]
-  \\ NTAC 3 (FULL_SIMP_TAC (srw_ss()) [Once (hd (tl (CONJUNCTS evaluate_cases)))])
-  \\ SIMP_TAC (srw_ss()) [Once evaluate_cases,PULL_EXISTS]
-  \\ FULL_SIMP_TAC (srw_ss()) [Once (hd (tl (CONJUNCTS evaluate_cases))),
-       evaluate_Lit,PULL_EXISTS]
-  \\ SIMP_TAC (srw_ss()) [Once evaluate_cases,PULL_EXISTS]
-  \\ FULL_SIMP_TAC (srw_ss()) [Once (hd (tl (CONJUNCTS evaluate_cases))),
-       evaluate_Lit,PULL_EXISTS]
-  \\ REPEAT STRIP_TAC
-  \\ SRW_TAC [] []
-  \\ IMP_RES_TAC do_app_IMP
-  \\ SRW_TAC [] []
-  \\ FULL_SIMP_TAC std_ss []
-  \\ FULL_SIMP_TAC (srw_ss()) [do_app_def]
-  \\ SRW_TAC [] []
-  \\ FULL_SIMP_TAC (srw_ss()) [opn_lookup_def, dest_binop_def,
-       intLib.COOPER_PROVE ``i + i2 - i2 = i:int``,
-       intLib.COOPER_PROVE ``i - i2 + i2 = i:int``]
-  \\ SRW_TAC [] [intLib.COOPER_PROVE ``x+y-y:int = x``,with_same_refs_io]);
+  \\ SIMP_TAC (srw_ss()) [evaluate_def]
+  >> every_case_tac
+  >> rw []
+  >> rw [state_component_equality]
+  >> fs []
+  >> rw []
+  >> fs [semanticPrimitivesPropsTheory.do_app_cases]
+  >> rw []
+  >> fs []
+  >> rw [opn_lookup_def]
+  >> intLib.ARITH_TAC);
 
 (* top-level optimiser *)
 
 val OPTIMISE_def = Define `
   OPTIMISE =
-    BOTTOM_UP_OPT (opt_sub_add o let_id) o BOTTOM_UP_OPT abs2let`;
+    BOTTOM_UP_OPT (opt_sub_add o let_id) (*o BOTTOM_UP_OPT abs2let*)`;
+
+val sing_opt_to_list = Q.prove (
+`(∀^s env exp t res.
+   evaluate s env [exp] = (t,Rval res) ⇒
+   evaluate s env [f exp] = (t,Rval res))
+ ⇒
+ (∀^s env exp t res.
+   evaluate s env exp = (t,Rval res) ⇒
+   evaluate s env (MAP f exp) = (t,Rval res))`,
+ strip_tac
+ >> Induct_on `exp`
+ >> rw []
+ >> pop_assum mp_tac
+ >> ONCE_REWRITE_TAC [evaluatePropsTheory.evaluate_cons]
+ >> every_case_tac
+ >> rw []
+ >> res_tac
+ >> fs []
+ >> rw []
+ >> fs []);
 
 val Eval_OPTIMISE = store_thm("Eval_OPTIMISE",
   ``Eval env exp P ==> Eval env (OPTIMISE exp) P``,
   SIMP_TAC std_ss [Eval_def] \\ REPEAT STRIP_TAC
   \\ Q.EXISTS_TAC `res` \\ FULL_SIMP_TAC std_ss [OPTIMISE_def]
+  \\ qexists_tac `k`
+  >> simp_tac std_ss [Once map_sing_lemma]
   \\ MATCH_MP_TAC BOTTOM_UP_OPT_THM
-  \\ SIMP_TAC std_ss [opt_sub_add_thm,let_id_thm]
+  >> simp []
+  >> match_mp_tac sing_opt_to_list
+  \\ SIMP_TAC std_ss [opt_sub_add_thm,let_id_thm]);
+
+  (*
   \\ MATCH_MP_TAC BOTTOM_UP_OPT_THM
   \\ ASM_SIMP_TAC std_ss [abs2let_thm]);
+  *)
 
 val _ = export_theory();
